#notes #math112 #math #calc



### quick worksheet aside
 4a. $$\int (2x)^{2}\cos(3x)dx$$
 - thiiiis is gonna need integration by parts
	 - $$u = (2x)^{2}$$
	 - we'll need a gross repeated integration by parts

###### example
$$\int x^{3}e^{3x}dx$$
$$u = x^{3,}dv = e^{3x}$$
$$du = 3x^{2}dx , v = \frac{1}{3}e^{3x}$$
$$x^{3}* \frac{1}{3}e^{3x}- \int3x^{2} \frac{1}{3}e^{3x}dx$$

| u        | dv                   |
| -------- | -------------------- |
| $x^3$    | $e^{3x}$             |
| $3x^{2}$ | $\frac{1}{3}e^{3x}$  |
| $6x$     | $\frac{1}{9}e^{3x}$  |
| $6$      | $\frac{1}{27}e^{3x}$ |
| $0$      | $\frac{1}{81}e^{3x}$ |
$$I = +\left(x^{3}* \frac{1}{3}e^{3x}\right)- (3x^{2}* \frac{1}{9}e^{3x})+ (6x  * \frac{1}{27}e^{3x})- ( 6 * \frac{1}{81}e^{3x})$$
There are two end cases - either you have to take a derivative of 0, or $I$ shows up again


----


### today's fresh torture

$$\frac{3x-1}{(x+1)(x-1)} = \frac{A}{(x-1)} + \frac{B}{(x+1)} = \frac{A(x+1)+B(x-1)}{(x-1)(x+1)}$$
- solving it the way we did yesterday is generally known as matching coefficients 
- This method is always gonna work, no if ands or buts about it, and it all makes sense

#### Method 2: Convenient Values of x
$$\frac{3x-1}{(x-1)(x+1)}(x-1)= A + \frac{B(1-1)}{1+1}$$
$$A = \frac{3(1)-1}{(1+1)}$$


----


$${\frac{(3x-1)}{(x-1)(x+1)} = \frac{A}{(x-1)}+\frac{B}{{(x+1)}}}$$
$$\frac{(3x-1)}{(x-1)\cancel{(x+1)}}\cancel{(x+1)} = \frac{A(x+1)}{(x-1)}+\frac{B}{\cancel{(x+1)}}\cancel{(x+1)}$$
$$\frac{3(-1)-1}{-1-1}= 0+B$$
$$B = 2$$

---

What happens if $$\frac{P(x)}{Q(x)}$$ is not proper?

If the degree of $p$ is the same or greater than that of the denominator

Say we have $$\frac{x^{3}-1}{{x^{2}-x}}$$
- We're uh, we're sent to long division hell.
$$x+1$$
$$x^{2}-x)\overline{x^{3}+0x^{2}+0x -1}$$
$$-(x^{3}-x^{2})$$
$$x^{2}+0x - ( x^{2}-x)$$$$+x -1 $$ is our remainder

$$\frac{x^{3}-1 }{x^{2}-x}= x+1 + \frac{x-1}{x^{2}-x}$$
Oh hey, now we're proper, so we can actually do partial fractions (isn't that neat)



### case 2 (the suffering never ends)
#### repeated linear factors

Now our denominator $Q(x)$, can be represented by $(x-a_{1})^{M_{1}}(x-a_{2})^{M_{2}}....(x-a_{n})^{M_{n}}$

Example: $Q(x)=x^{2}(x-1)$
$$Q = (x-0)^{2}(x-1)^{1}$$$$a_{1}= 0, m_{1}= 2$$$$a_{2}= 1, M_{2}= 1$$
$$\text{ For each (x-a)}^{M}\newline \text{ we will use } (\frac{A_1}{(x-a)^{1}})+(\frac{A_2}{(x-a)^{2}})+....(\frac{A_{M}}{(x-a)^{M}})$$

$$\frac{P(x)}{Q(x)}=\frac{x^{2}-x +3 }{x^{2}(x-1)}= \frac{A_{1}}{(x-0)^{1}}+ \frac{A_2}{(x-0)^{2}} + \frac{B}{x-1}$$
$$B = \frac{x^{2}-x+3}{x^{2}}, = \frac{1-1+3}{1^{2}}=3$$
- Here we multiplied everything by $(x-1)$, the linear factor associated with $B$

$$A_{2}= \frac{x^{2}-x+3}{x-1}\rvert_{0}, A_{2}= -3$$
- Multiplied everything by x^2 
- go home and find $A_{1}$
- 